src/SDK/CMM/Defs.dfy
@@ -18,7 +18,6 @@ module CMMDefs {
                                   returns (res: Result<Materials.ValidEncryptionMaterialsOutput>)
       requires Valid()
       ensures Valid()
-      ensures res.Success? && algSuiteID.Some? ==> res.value.dataKey.algorithmSuiteID == algSuiteID.get
 
     method DecryptMaterials(algSuiteID: AlgorithmSuite.ID,
                             edks: seq<Materials.EncryptedDataKey>,
@@ -27,6 +26,5 @@ module CMMDefs {
       requires |edks| > 0
       requires Valid()
       ensures Valid()
-      ensures res.Success? ==> res.value.dataKey.algorithmSuiteID == algSuiteID
   }
 }
